\documentclass[]{article}
\usepackage{amsmath}
\usepackage{amsfonts}
\usepackage{amssymb}
\usepackage{algorithmic}
\usepackage{algorithm}
\usepackage{tikz}
\usepackage{graphicx}
\usepackage{mdframed}
\usepackage{paralist}

\title{CAGD - Homework 1}
\author{Josefine St√•l \& Erik Ackzell}

\begin{document}

\maketitle

\section*{Task 3}
We want to show that linear interpolation $\Phi : \mathbb{R} \mapsto \mathbb{E}^2$ is an affine map.\\
\underline{\textbf{Proof:}} Let $p,q$ be arbitrary points in $\mathbb{E}^2$. Then \begin{equation*}
\Phi (t) = (1-t)p + tq, \quad t\in \mathbb{R}
\end{equation*}
is the linear interpolation of $p$ and $q$. Let $x\in \mathbb{R}$ be a barycentric combination, i.e. $x=\sum_{i=1}^{n}\alpha_i x_i$ with $x_i, \alpha_i\in \mathbb{R}$ and $\sum_{i=1}^{n}\alpha_i = 1$. Then \begin{equation*}
\begin{aligned}
\Phi (x) &= \Phi (\sum_{i=1}^{n}\alpha_i x_i)\\
&=(1-\sum_{i=1}^{n}\alpha_i x_i)p + (\sum_{i=1}^{n}\alpha_i x_i)p\\
&\overset{(i)}{=}(\sum_{i=1}^{n}\alpha_i-\sum_{i=1}^{n}\alpha_i x_i)p + \sum_{i=1}^{n}\alpha_i x_ip\\
&=\sum_{i=1}^{n}\alpha_i[(1-x_i)p + x_iq]\\
&=\sum_{i=1}^{n}\alpha_i\Phi(x_i)
\end{aligned}
\end{equation*}
where $(i)$ follows from $\sum_{i=1}^{n}\alpha_i=1$. This is what we wanted to show. $\square$
\end{document}
